MonadCOP.v
@@ -5,6 +5,9 @@ Require Import ExtLib.Data.Monads.StateMonad ExtLib.Data.Monads.ReaderMonad ExtL
 Require Import List.
 Import ListNotations.
 
+Import MonadNotation.
+Local Open Scope monad_scope.
+
 Record Cop_Env : Type := mkCop_Env
                            { nameServer : NS ;
                              me : Plc}.
@@ -17,3 +20,10 @@ Definition runCOP {A:Type} (k:(COP A)) (env:Cop_Env) : A (* (A * AM_St)*) :=
   unIdent (runReaderT k env).
 
 Definition empty_cop_env := (mkCop_Env [] 0).
+
+
+Fixpoint foldM_COP {A B : Type} (f:A -> B -> COP A) (a:A) (bs:list B) : COP A :=
+  match bs with
+  | [] => ret a
+  | (x::xs) => f a x >>= fun fax => foldM_COP f fax xs
+  end.
